update spec equiv proof of gf128

code/experimental/gf128/Hacl.Spec.Gf128.FieldNI.fst
@@ -169,15 +169,15 @@ let gf128_reduce (hi:vec128) (lo:vec128) : Tot vec128 =
   lo
 
 
-val gf128_clmud_wide_reduce_lemma: x:vec128 -> y:vec128 -> Lemma
+val gf128_clmul_wide_reduce_lemma: x:vec128 -> y:vec128 -> Lemma
   (let (hi, lo) = clmul_wide x y in
    to_elem (gf128_reduce hi lo) == GF.fmul_be #S.gf128 (to_elem x) (to_elem y))
-let gf128_clmud_wide_reduce_lemma x y = admit()
+let gf128_clmul_wide_reduce_lemma x y = admit()
 
 
-val gf128_clmud_wide4_reduce_lemma:
+val gf128_clmul_wide4_reduce_lemma:
     x1:vec128 -> x2:vec128 -> x3:vec128 -> x4:vec128
   -> y1:vec128 -> y2:vec128 -> y3:vec128 -> y4:vec128 -> Lemma
   (let (hi, lo) = clmul_wide4 x1 x2 x3 x4 y1 y2 y3 y4 in
    to_elem (gf128_reduce hi lo) == Vec.normalize4 (to_elem4 y1 y2 y3 y4) (to_elem4 x1 x2 x3 x4))
-let gf128_clmud_wide4_reduce_lemma x1 x2 x3 x4 y1 y2 y3 y4 = admit()
+let gf128_clmul_wide4_reduce_lemma x1 x2 x3 x4 y1 y2 y3 y4 = admit()
